Fix (some) Vale tests
These have been disabled since long ago. Restore some of them.

tests/vale/TransparentMap.fst
@@ -37,23 +37,23 @@ let sel_upd2 (#k:eqtype) (#v:Type) (m:map k v) (key1:k) (key2:k) (value:v)
     [SMTPat (sel (upd m key1 value) key2)]
   = ()
 
-abstract type equal (#key:eqtype) (#value:Type) (m1: map key value) (m2: map key value) =
+type equal (#key:eqtype) (#value:Type) (m1: map key value) (m2: map key value) =
   feq m1 m2
 
-abstract val lemma_equal_intro: #key:eqtype -> #value:Type -> m1:map key value -> m2:map key value ->
+val lemma_equal_intro: #key:eqtype -> #value:Type -> m1:map key value -> m2:map key value ->
                        Lemma (requires (forall k. sel m1 k == sel m2 k))
                        (ensures (equal m1 m2))
                        [SMTPat (equal m1 m2)]
 
 
 
-abstract val lemma_equal_elim: #key:eqtype -> #value:Type -> m1:map key value -> m2:map key value ->
+val lemma_equal_elim: #key:eqtype -> #value:Type -> m1:map key value -> m2:map key value ->
                       Lemma (requires (equal m1 m2)) (ensures  (m1 == m2))
                       [SMTPat (equal m1 m2)]
 
 
 
-abstract val lemma_equal_refl: #key:eqtype -> #value:Type -> m1:map key value -> m2:map key value ->
+val lemma_equal_refl: #key:eqtype -> #value:Type -> m1:map key value -> m2:map key value ->
                       Lemma  (requires (m1 == m2)) (ensures  (equal m1 m2))
 		      [SMTPat (equal m1 m2)]
 
