tests/vale/X64.Vale.State_i.fsti
@@ -16,6 +16,8 @@
 module X64.Vale.State_i
 // This interface should not refer to Semantics_s
 
+module F = FStar.FunctionalExtensionality
+
 open X64.Machine_s
 open X64.Vale
 
@@ -64,7 +66,7 @@ let eval_operand (o:operand) (s:state) : nat64 =
   | OMem m -> eval_mem (eval_maddr m s) s
 
 let update_reg (r:reg) (v:nat64) (s:state) : state =
-  { s with regs = fun r' -> if  r = r' then v else s.regs r' }
+  { s with regs = F.on_domain _ (fun r' -> if  r = r' then v else s.regs r') }
 
 let update_mem (ptr:int) (v:nat64) (s:state) : state = { s with mem = Map.upd s.mem ptr v }
 
